verify/IndSBCv1.v
@@ -1,0 +1,257 @@
+From BusyCoq Require Import Individual62.
+Require Import Lia.
+Require Import ZArith.
+Require Import String.
+From BusyCoq Require Import Inductive.
+
+Module Inductive62 := Inductive BB62.
+Import Inductive62.
+
+Lemma progress_rw tm c1 c2:
+  progress tm c1 c2 <->
+  Compute.TM.progress tm c1 c2.
+Proof.
+  split; intro H.
+  - induction H.
+    + constructor.
+      destruct H; auto.
+    + eapply Compute.TM.progress_step; eauto.
+      destruct H; auto.
+  - induction H.
+    + constructor.
+      destruct H; auto.
+    + eapply progress_step; eauto.
+      destruct H; auto.
+Qed.
+
+Ltac solve_rule :=
+  unfold Config_WF; cbn;
+  repeat rewrite List.Forall_cons_iff;
+  repeat rewrite List.Forall_nil_iff;
+  cbn;
+  repeat split;
+  intros;
+  unfold s0;
+  rewrite progress_rw;
+  try (es; fail).
+
+Ltac solve_hlin_nonhalt_T cfg T :=
+  apply (decide_hlin_nonhalt_spec cfg T);
+  [ solve_rule
+  | vm_cast_no_check (eq_refl true)].
+
+Ltac solve_hlin_nonhalt cfg :=
+  match goal with
+  | |- ~halts (TM_from_str ?x) c0 =>
+    idtac x;
+    (solve_hlin_nonhalt_T cfg 200000%N)
+  end.
+
+
+Lemma nonhalt1: ~halts (TM_from_str "1LB1LF_1LC0LA_0RD1RA_1LE1RD_1LD0RC_---1RE") c0.
+Proof. solve_hlin_nonhalt (config_SBC 7450%N 5 A A A A [0] [1] [0;1;0] [1] [0;0;0;1] [0;1;0;1] [0;1;0]). Time Qed.
+
+Lemma nonhalt2: ~halts (TM_from_str "1LB1LF_1LC0LA_0RD1RA_1LE1RD_1LE0RC_---1RE") c0.
+Proof. solve_hlin_nonhalt (config_SBC 7450%N 5 A A A A [0] [1] [0;1;0] [1] [0;0;0;1] [0;1;0;1] [0;1;0]). Time Qed.
+
+Lemma nonhalt3: ~halts (TM_from_str "1LB---_0LC1RE_0RD1LF_1LC1RB_0RF0RA_0LA0RB") c0.
+Proof. solve_hlin_nonhalt (config_SBC 5604%N 3 A B A B [0] [1] [0;1;0] [1] [0;0;1;1] [0;0;1;0] [0]). Time Qed.
+
+Lemma nonhalt4: ~halts (TM_from_str "1RB1LB_0LC0RE_1LE0RD_1RE---_0LA1RF_0RB0RC") c0.
+Proof. solve_hlin_nonhalt (config_SBC 5659%N 3 C E C E [0] [1] [0;1;0] [1] [0;0;1;1] [0;0;1;0] [0]). Time Qed.
+
+Lemma nonhalt5: ~halts (TM_from_str "1RB---_0LC1RF_0RA1LD_0LE0RB_1LB---_0RD0RE") c0.
+Proof. solve_hlin_nonhalt (config_SBC 5502%N 3 E B E B [0] [1] [0;1;0] [1] [0;0;1;1] [0;0;1;0] [0]). Time Qed.
+
+Lemma nonhalt6: ~halts (TM_from_str "1RB1RF_0LC1RF_0RA1LD_0LE0RA_1LB---_0RD0RE") c0.
+Proof. solve_hlin_nonhalt (config_SBC 5358%N 3 E A E A [] [] [0;1] [] [0;0;1;1] [0;0;1;0] [0]). Time Qed.
+
+Lemma nonhalt7: ~halts (TM_from_str "1RB1RF_0LC1RF_1LF1LD_0LE0RA_1LB---_0RD0RE") c0.
+Proof. solve_hlin_nonhalt (config_SBC 1585%N 3 B D B D [] [] [1;0] [] [0;1;1;0] [0;1;0;0] [0]). Time Qed.
+
+Lemma nonhalt8: ~halts (TM_from_str "1LB---_1LC0LA_0RD1RE_1LE1RD_1LF0RC_0LD0LA") c0.
+Proof. solve_hlin_nonhalt (config_SBC 6188%N 5 A E A E [0] [1] [0;1;0] [1] [0;0;0;1] [0;1;0;1] [0;1;0]). Time Qed.
+
+Lemma nonhalt9: ~halts (TM_from_str "1LB---_1LC0LA_0RD1RE_1LE1RD_1LF0RC_1LE0LA") c0.
+Proof. solve_hlin_nonhalt (config_SBC 6158%N 5 A E A E [0] [1] [0;1;0] [1] [0;0;0;1] [0;1;0;1] [0;1;0]). Time Qed.
+
+Lemma nonhalt10: ~halts (TM_from_str "1LB---_1LC0LA_0RD1RF_1LE1RD_1LD0RC_1LB0RC") c0.
+Proof. solve_hlin_nonhalt (config_SBC 6158%N 5 A F A F [0] [1] [0;1;0] [1] [0;0;0;1] [0;1;0;1] [0;1;0]). Time Qed.
+
+Lemma nonhalt11: ~halts (TM_from_str "1LB0RC_1LC0LF_0RD1RA_1LE1RD_1LE0RC_1LB---") c0.
+Proof. solve_hlin_nonhalt (config_SBC 6158%N 5 F A F A [0] [1] [0;1;0] [1] [0;0;0;1] [0;1;0;1] [0;1;0]). Time Qed.
+
+Lemma nonhalt12: ~halts (TM_from_str "1RB1LD_1RC0RB_1LA1RF_0LC1LE_0RF---_0RD0RA") c0.
+Proof. solve_hlin_nonhalt (config_SBC 3476%N 5 E B E B [1;1] [0;1] [1;1;1;0;1] [0;1] [0;1;1;0;0;1] [0;1;1;0;1;1] [0;1;1;0;1]). Time Qed.
+
+Lemma nonhalt13: ~halts (TM_from_str "1RB1LD_1RC0RB_1LA1RF_0LC1RE_---1LF_0RD0RA") c0.
+Proof. solve_hlin_nonhalt (config_SBC 3480%N 5 C B C B [0;1] [0;1] [0;1;1;0;1] [0;1] [0;1;1;0;0;1] [0;1;1;0;1;1] [0;1;1;0;1]). Time Qed.
+
+Lemma nonhalt14: ~halts (TM_from_str "1RB---_1LC0RD_1RD0LC_0RE0LF_0LB1RF_0RB1RA") c0.
+Proof. solve_hlin_nonhalt (config_SBC 1831%N 5 C B C B [0;1;0] [0;1;0] [0;1;0;1;0] [0;1;0] [0;0;1;0] [1;0;1;0] [1]). Time Qed.
+
+Lemma nonhalt15: ~halts (TM_from_str "1LB0RF_1RC0LB_0RD1RA_0LA1RE_1LD0RA_0RD---") c0.
+Proof. solve_hlin_nonhalt (config_SBC 1839%N 5 B A B A [0;1;0] [0;1;0] [0;1;0;1;0] [0;1;0] [0;0;1;0] [1;0;1;0] [1]). Time Qed.
+
+Lemma nonhalt16: ~halts (TM_from_str "1LB1RA_1RC0LE_1RE0RD_0RC1RF_0LA0RA_0LB---") c0.
+Proof. solve_hlin_nonhalt (config_SBC 2126%N 4 E C E C [0;1;0] [0;0;1] [0;1;0;1;0;0] [0;0;1] [1;0;0;0;0;1] [1;0;0;1;0;1] [1;0;0;1]). Time Qed.
+
+Lemma nonhalt17: ~halts (TM_from_str "1RB0LA_0LC0RC_0RE0RD_1RE---_1LF0RA_0LA0LE") c0.
+Proof. solve_hlin_nonhalt (config_SBC 1268%N 5 E A E A [] [] [0;1] [] [0;0;0;1] [0;1;0;1] [0;1;0]). Time Qed.
+
+Lemma nonhalt18: ~halts (TM_from_str "1RB1RC_1LC0RE_1LD0RA_0LA0LC_0RC0RF_0LA---") c0.
+Proof. solve_hlin_nonhalt (config_SBC 5188%N 5 C A C A [] [] [0;1] [] [0;0;0;1] [0;1;0;1] [0;1;0]). Time Qed.
+
+Lemma nonhalt19: ~halts (TM_from_str "1LB1RE_1RC1LD_1RA0RC_0LA0LE_0RD0RF_1RC---") c0.
+Proof. solve_hlin_nonhalt (config_SBC 769%N 5 E C E F [0] [1] [0;1;1] [] [0;1;1;0;0;1] [0;1;1;0;1;1] [0;1;1;0;1]). Time Qed.
+
+Lemma nonhalt20: ~halts (TM_from_str "1LB1RE_1RC1LD_1RA0RC_0LA0LF_0RD0RB_0RD---") c0.
+Proof. solve_hlin_nonhalt (config_SBC 769%N 5 F C F B [0] [1] [0;1;1] [] [0;1;1;0;0;1] [0;1;1;0;1;1] [0;1;1;0;1]). Time Qed.
+
+Lemma nonhalt21: ~halts (TM_from_str "1RB0LD_0RC0RF_1RD0RA_1LE0RC_1LA1LE_---1RC") c0.
+Proof. solve_hlin_nonhalt (config_SBC 3076%N 4 E F E F [] [] [1;0;1] [] [0;1;0;0;1;1] [0;1;0;0;1;0] [0;1]). Time Qed.
+
+Lemma nonhalt22: ~halts (TM_from_str "1RB0RA_1LC1RE_1RA1LD_0LB0RF_0RD0RC_---1LD") c0.
+Proof. solve_hlin_nonhalt (config_SBC 788%N 5 B C B C [] [] [0;1;1] [] [0;1;1;0;0;1] [0;1;1;0;1;1] [0;1;1;0;1]). Time Qed.
+
+Lemma nonhalt23: ~halts (TM_from_str "1RB1LD_1RC0RB_1LA1RE_0LC0LE_0RD0RF_1RB---") c0.
+Proof. solve_hlin_nonhalt (config_SBC 789%N 5 E B E F [0] [1] [0;1;1] [] [0;1;1;0;0;1] [0;1;1;0;1;1] [0;1;1;0;1]). Time Qed.
+
+Lemma nonhalt24: ~halts (TM_from_str "1RB1LD_1RC0RB_1LA1RF_0LC0LE_0RD---_0RD0RA") c0.
+Proof. solve_hlin_nonhalt (config_SBC 789%N 5 E B E A [0] [1] [0;1;1] [] [0;1;1;0;0;1] [0;1;1;0;1;1] [0;1;1;0;1]). Time Qed.
+
+Lemma nonhalt25: ~halts (TM_from_str "1RB0LA_0RC1RD_0LD1RE_1LA0RB_0RD0RF_1LA---") c0.
+Proof. solve_hlin_nonhalt (config_SBC 483%N 5 A D A C [0;1;0] [0;1;0] [0;1;0] [0] [0;0;1;0] [1;0;1;0] [1]). Time Qed.
+
+Lemma nonhalt26: ~halts (TM_from_str "1RB0LA_0RC1RD_0LD1RE_1LA0RB_0RD0RF_0LE---") c0.
+Proof. solve_hlin_nonhalt (config_SBC 485%N 5 A D A C [0;1;0] [0;1;0] [0;1;0] [0] [0;0;1;0] [1;0;1;0] [1]). Time Qed.
+
+Lemma nonhalt27: ~halts (TM_from_str "1RB1RA_0RC0RF_0LD---_1LE1RE_0RD1LF_1RA0LD") c0.
+Proof. solve_hlin_nonhalt (config_SBC 2249%N 5 F F F B [1;1] [0;1] [1;1;0] [1] [1;1;0;1] [1;1;1;1] [1;1;1]). Time Qed.
+
+Lemma nonhalt28: ~halts (TM_from_str "1RB0LE_1RC1RB_1RD0RA_1LC---_1LF1RF_0RE1LA") c0.
+Proof. solve_hlin_nonhalt (config_SBC 2304%N 5 A A A C [1;1] [0;1] [1;1;0] [1] [1;1;0;1] [1;1;1;1] [1;1;1]). Time Qed.
+
+Lemma nonhalt29: ~halts (TM_from_str "1LB1RE_0LC0LB_1RD1LB_0RA---_0RF0LB_1RA0RD") c0.
+Proof. solve_hlin_nonhalt (config_SBC 465%N 3 B A B A [] [] [1;0] [] [0;0;0;1] [0;1;0;1] [0;1]). Time Qed.
+
+Lemma nonhalt30: ~halts (TM_from_str "1RB1RC_1LC0RE_1LD0RA_0LA0LC_0RC1RF_1LC---") c0.
+Proof. solve_hlin_nonhalt (config_SBC 4660%N 5 C A C A [] [] [0;1] [] [0;0;0;1] [0;1;0;1] [0;1;0]). Time Qed.
+
+Lemma nonhalt31: ~halts (TM_from_str "1RB1RE_0LC0RC_0RE1RD_1LE---_1LF0RA_0LA0LE") c0.
+Proof. solve_hlin_nonhalt (config_SBC 4800%N 5 E A E A [] [] [0;1] [] [0;0;0;1] [0;1;0;1] [0;1;0]). Time Qed.
+
+Lemma nonhalt32: ~halts (TM_from_str "1RB1LC_1LA1RD_0LB1LA_0RE1RF_---0RA_0RA0RB") c0.
+Proof. solve_hlin_nonhalt (config_SBC 2343%N 6 A F A D [1] [1] [1;1] [] [1;0;1;1;0;1] [1;1;1;1;1;1] [1;1;1;1;1]). Time Qed.
+
+Lemma nonhalt33: ~halts (TM_from_str "1LB1RA_1RC0LE_1RE0RD_0RC0RF_0LA0RA_0LE---") c0.
+Proof. solve_hlin_nonhalt (config_SBC 1950%N 4 E C E E [0;1;0] [0;0;1] [0;1;0] [] [1;0;0;0;0;1] [1;0;0;1;0;1] [1;0;0;1]). Time Qed.
+
+Lemma nonhalt34: ~halts (TM_from_str "1LB1RF_1RC0LE_1RE0RD_0RC0LE_0LA0RA_1LB---") c0.
+Proof. solve_hlin_nonhalt (config_SBC 1950%N 4 E D E E [0;1] [0;1] [0;1;0] [] [1;0;0;0;0;1] [1;0;0;1;0;1] [1;0;0;1]). Time Qed.
+
+Lemma nonhalt35: ~halts (TM_from_str "1LB1RF_1RC0LE_1RE0RD_0RC0LE_0LA0RA_1LD---") c0.
+Proof. solve_hlin_nonhalt (config_SBC 1950%N 4 E D E E [0;1] [0;1] [0;1;0] [] [1;0;0;0;0;1] [1;0;0;1;0;1] [1;0;0;1]). Time Qed.
+
+Lemma nonhalt36: ~halts (TM_from_str "1LB1RE_0LC0LB_1RD1LB_0RA---_0RF1RF_1RA0RD") c0.
+Proof. solve_hlin_nonhalt (config_SBC 2085%N 3 B A B A [] [] [1;0] [] [0;0;0;1] [0;1;0;1] [0;1]). Time Qed.
+
+Lemma nonhalt37: ~halts (TM_from_str "1LB0RC_1RC0LB_0RD1RA_0LA1RE_0RA1RF_1RB---") c0.
+Proof. solve_hlin_nonhalt (config_SBC 1447%N 5 B D B C [0] [0] [0;1] [] [0;0;1;0] [1;0;1;0] [1]). Time Qed.
+
+Lemma nonhalt38: ~halts (TM_from_str "1RB1LD_0RC---_1LD1RE_0LA0LD_0RF0LD_1RC0RB") c0.
+Proof. solve_hlin_nonhalt (config_SBC 615%N 3 D C D C [] [] [1;0] [] [0;0;0;1] [0;1;0;1] [0;1]). Time Qed.
+
+Lemma nonhalt39: ~halts (TM_from_str "1RB1LD_0RC---_1LD1RE_0LA0LD_0RF1RF_1RC0RB") c0.
+Proof. solve_hlin_nonhalt (config_SBC 769%N 3 D C D C [] [] [1;0] [] [0;0;0;1] [0;1;0;1] [0;1]). Time Qed.
+
+Lemma nonhalt40: ~halts (TM_from_str "1LB0RD_1LC1RE_1RA0LB_1RE1RB_0RC0RF_0RA---") c0.
+Proof. solve_hlin_nonhalt (config_SBC 2482%N 8 C A C E [1;0] [0;0] [1;0] [] [1;0;0;0] [1;0;1;0] [1;0;1]). Time Qed.
+
+Lemma nonhalt41: ~halts (TM_from_str "1RB0RE_1RC1RF_1LD0LC_1RE1LC_1LB0RB_---0RA") c0.
+Proof. solve_hlin_nonhalt (config_SBC 762%N 3 D F D F [] [] [1;1] [] [1;0;0;0] [1;0;1;0] [1;0;1]). Time Qed.
+
+Lemma nonhalt42: ~halts (TM_from_str "1RB0LA_0RC1RD_0LD1RE_1LA0RB_0RD1RF_1RA---") c0.
+Proof. solve_hlin_nonhalt (config_SBC 5007%N 5 A C A B [0] [0] [0;1] [] [0;0;1;0] [1;0;1;0] [1]). Time Qed.
+
+Lemma nonhalt43: ~halts (TM_from_str "1RB0LB_0RC1LD_1LD1RA_0LA0RE_0RC1RF_0RD---") c0.
+Proof. solve_hlin_nonhalt (config_SBC 1237%N 3 B A B C [0] [1] [0;0;1;0] [] [0;0;0;1;0;1] [0;1;0;1;0;1] [0;1]). Time Qed.
+
+Lemma nonhalt44: ~halts (TM_from_str "1LB1RC_0LC0RE_1RD0LD_0RA1LB_0RA1RF_0RB---") c0.
+Proof. solve_hlin_nonhalt (config_SBC 3725%N 3 D C D A [0] [1] [0;0;1;0] [] [0;0;0;1;0;1] [0;1;0;1;0;1] [0;1]). Time Qed.
+
+Lemma nonhalt45: ~halts (TM_from_str "1LB0LC_1RC1LE_0RD0RB_1RA1RF_0LF---_0LA0RC") c0.
+Proof. solve_hlin_nonhalt (config_SBC 4518%N 3 A B A B [] [] [0;0;1;1] [] [0;1;0;0;0;1;0;1] [0;1;0;0;0;1;0;0] [0;1]). Time Qed.
+
+Lemma nonhalt46: ~halts (TM_from_str "1RB1RE_1LC0LF_1RF1LD_0LE---_0LB0RF_0RA0RC") c0.
+Proof. solve_hlin_nonhalt (config_SBC 4643%N 3 B C B C [] [] [0;0;1;1] [] [0;1;0;0;0;1;0;1] [0;1;0;0;0;1;0;0] [0;1]). Time Qed.
+
+Lemma nonhalt47: ~halts (TM_from_str "1RB---_1LC0RD_0LD0LB_1RE1RB_1LB0RF_0RB0RA") c0.
+Proof. solve_hlin_nonhalt (config_SBC 4129%N 5 B D B D [] [] [0;1] [] [0;0;0;1] [0;1;0;1] [0;1;0]). Time Qed.
+
+Lemma nonhalt48: ~halts (TM_from_str "1RB---_1LC0RD_0LD0LB_1RE1RB_0LF0RF_0RB0RA") c0.
+Proof. solve_hlin_nonhalt (config_SBC 4129%N 5 B D B D [] [] [0;1] [] [0;0;0;1] [0;1;0;1] [0;1;0]). Time Qed.
+
+Lemma nonhalt49: ~halts (TM_from_str "1RB1LC_1LA1RD_0LB1LA_0RE1RF_---0LB_0RA0RB") c0.
+Proof. solve_hlin_nonhalt (config_SBC 1948%N 6 A D A D [] [] [1;1] [] [1;0;1;1;0;1] [1;1;1;1;1;1] [1;1;1;1;1]). Time Qed.
+
+Lemma nonhalt50: ~halts (TM_from_str "1RB1LC_1LA1RD_0LB1LA_1RE1RF_---0LC_0RA0RB") c0.
+Proof. solve_hlin_nonhalt (config_SBC 1948%N 6 A D A D [] [] [1;1] [] [1;0;1;1;0;1] [1;1;1;1;1;1] [1;1;1;1;1]). Time Qed.
+
+Lemma nonhalt51: ~halts (TM_from_str "1LB---_1RC0LE_1RE0RD_0RC0LA_0LF0RF_1LB1RA") c0.
+Proof. solve_hlin_nonhalt (config_SBC 1670%N 4 E D E E [0;1] [0;1] [0;1;0] [] [1;0;0;0;0;1] [1;0;0;1;0;1] [1;0;0;1]). Time Qed.
+
+Lemma nonhalt52: ~halts (TM_from_str "1LB---_1RC0LE_1RE0RD_0RC0LF_0LF0RF_1LB1RA") c0.
+Proof. solve_hlin_nonhalt (config_SBC 1670%N 4 E D E E [0;1] [0;1] [0;1;0] [] [1;0;0;0;0;1] [1;0;0;1;0;1] [1;0;0;1]). Time Qed.
+
+Lemma nonhalt53: ~halts (TM_from_str "1RB0RD_0RC0RB_0LD1RA_1LE---_0LF0RB_0LA1LC") c0.
+Proof. solve_hlin_nonhalt (config_SBC 2074%N 5 C C C C [] [] [1;0] [] [0;0;1;1] [0;0;0;1] [0;0;0]). Time Qed.
+
+Lemma nonhalt54: ~halts (TM_from_str "1LB1RE_1RC1LD_1RA0RC_0LA0LA_0RD0RF_1RC---") c0.
+Proof. solve_hlin_nonhalt (config_SBC 1918%N 5 A F A F [] [] [0;1;1] [] [0;1;1;0;0;1] [0;1;1;0;1;1] [0;1;1;0;1]). Time Qed.
+
+Lemma nonhalt55: ~halts (TM_from_str "1LB1RE_1RC1LD_1RA0RC_0LA0LF_0RD0RB_1LB---") c0.
+Proof. solve_hlin_nonhalt (config_SBC 1918%N 5 F B F B [] [] [0;1;1] [] [0;1;1;0;0;1] [0;1;1;0;1;1] [0;1;1;0;1]). Time Qed.
+
+Lemma nonhalt56: ~halts (TM_from_str "1RB1LD_1RC0RB_1LA1RE_0LC0LC_0RD0RF_1RB---") c0.
+Proof. solve_hlin_nonhalt (config_SBC 2074%N 5 C F C F [] [] [0;1;1] [] [0;1;1;0;0;1] [0;1;1;0;1;1] [0;1;1;0;1]). Time Qed.
+
+Lemma nonhalt57: ~halts (TM_from_str "1RB1LD_1RC0RB_1LA1RF_0LC0LE_1LA---_0RD0RA") c0.
+Proof. solve_hlin_nonhalt (config_SBC 2074%N 5 E A E A [] [] [0;1;1] [] [0;1;1;0;0;1] [0;1;1;0;1;1] [0;1;1;0;1]). Time Qed.
+
+Lemma nonhalt58: ~halts (TM_from_str "1RB0LD_1RC1LA_1RD0RC_1LB1RE_0RA0RF_1RC---") c0.
+Proof. solve_hlin_nonhalt (config_SBC 2074%N 5 D F D F [] [] [0;1;1] [] [0;1;1;0;0;1] [0;1;1;0;1;1] [0;1;1;0;1]). Time Qed.
+
+Lemma nonhalt59: ~halts (TM_from_str "1RB0RA_1LC1RE_1RA1LD_1RC0LB_0RD0RF_1RA---") c0.
+Proof. solve_hlin_nonhalt (config_SBC 2347%N 5 B F B F [] [] [0;1;1] [] [0;1;1;0;0;1] [0;1;1;0;1;1] [0;1;1;0;1]). Time Qed.
+
+Lemma nonhalt60: ~halts (TM_from_str "1RB1RF_0RC0RA_1RD0LE_1LC1RA_1LC1LE_---0RB") c0.
+Proof. solve_hlin_nonhalt (config_SBC 2789%N 2 E A E C [] [] [0] [] [0;0;1] [1;1;1] [1;1]). Time Qed.
+
+Lemma nonhalt61: ~halts (TM_from_str "1RB0LC_1LA1RD_1LA1LC_1RE1RF_0RA0RD_---0RE") c0.
+Proof. solve_hlin_nonhalt (config_SBC 2767%N 2 C D C A [] [] [0] [] [0;0;1] [1;1;1] [1;1]). Time Qed.
+
+Lemma nonhalt62: ~halts (TM_from_str "1RB0RF_0RC0RA_1RD0LE_1LC1RA_1LC1RD_---1RB") c0.
+Proof. solve_hlin_nonhalt (config_SBC 3015%N 2 E B E B [0] [1] [0;1] [1] [0;0;1] [1;1;1] [1;1]). Time Qed.
+
+Lemma nonhalt63: ~halts (TM_from_str "1RB0RF_0RC0RA_1RD0LE_1LC1RA_1LC1RE_---1RB") c0.
+Proof. solve_hlin_nonhalt (config_SBC 3015%N 2 E B E B [0] [1] [0;1] [1] [0;0;1] [1;1;1] [1;1]). Time Qed.
+
+Lemma nonhalt64: ~halts (TM_from_str "1RB0RF_0RC0RA_1RD0LE_0LE1RA_1LC1RE_---1RB") c0.
+Proof. solve_hlin_nonhalt (config_SBC 3057%N 2 E B E B [0] [1] [0;1] [1] [0;0;1] [1;1;1] [1;1]). Time Qed.
+
+Lemma nonhalt65: ~halts (TM_from_str "1RB1RF_0RC0RA_1RD0LE_1LC1RA_1LC1RD_---0LB") c0.
+Proof. solve_hlin_nonhalt (config_SBC 3109%N 2 E B E B [0] [1] [0;1] [1] [0;0;1] [1;1;1] [1;1]). Time Qed.
+
+Lemma nonhalt66: ~halts (TM_from_str "1RB1RF_0RC0RA_1RD0LE_1LC1RA_1LC1RE_---0LB") c0.
+Proof. solve_hlin_nonhalt (config_SBC 3109%N 2 E B E B [0] [1] [0;1] [1] [0;0;1] [1;1;1] [1;1]). Time Qed.
+
+Lemma nonhalt67: ~halts (TM_from_str "1RB1RF_0RC0RA_1RD0LE_0LE1RA_1LC1RE_---0LB") c0.
+Proof. solve_hlin_nonhalt (config_SBC 3151%N 2 E B E B [0] [1] [0;1] [1] [0;0;1] [1;1;1] [1;1]). Time Qed.
+
+Lemma nonhalt68: ~halts (TM_from_str "1LB1RF_1RC1RA_1RE0RD_0RC0LE_0LA0RA_1LD---") c0.
+Proof. solve_hlin_nonhalt (config_SBC 2710%N 4 E D E E [0;1] [0;1] [0;1;0] [] [1;0;0;0;0;1] [1;0;0;1;0;1] [1;0;0;1]). Time Qed.
+
+Lemma nonhalt69: ~halts (TM_from_str "1RB0RC_1RC0LC_0RD0LE_1LE1RF_0LB---_0RA0LA") c0.
+Proof. solve_hlin_nonhalt (config_SBC 2093%N 5 C F C D [0] [1] [0;0] [] [0;0;0;1] [0;1;0;1] [0;1]). Time Qed.
+
